From30To40/Translate.v
@@ -1,4 +1,4 @@
-From Coq Require Import ZArith NArith String.
+From Coq Require Import ZArith NArith String Lia.
 
 From Vyper Require Import Config NaryFun.
 From Vyper Require L30.AST L40.AST.
@@ -50,7 +50,7 @@ Definition BuiltinsSupportStorage {C: VyperConfig}
 
 
 
-Local Definition var_range {C: VyperConfig} (offset count: N)
+Definition var_range {C: VyperConfig} (offset count: N)
 : list L40.AST.expr
 := let fix var_range' (countdown: nat)
    := match countdown with
@@ -66,7 +66,83 @@ Proof.
 trivial.
 Qed.
 
-Definition translate_small_stmt {C: VyperConfig} (B: builtin_names_config) (ss: L30.AST.small_stmt)
+Definition var_range_nat {C: VyperConfig} (offset count: nat)
+: list L40.AST.expr
+:= let fix var_range' (countdown: nat)
+   := match countdown with
+      | O => nil
+      | S k => cons (L40.AST.LocalVar (N.of_nat (offset + count - 1 - k)))
+                    (var_range' k)
+      end
+   in var_range' count.
+
+Lemma var_range_nat_ok {C: VyperConfig} (offset count: nat):
+  var_range_nat offset count = var_range (N.of_nat offset) (N.of_nat count).
+Proof.
+unfold var_range, var_range_nat.
+rewrite Nat2N.id.
+revert offset. induction count. { trivial. }
+intro offset. cbn.
+assert (IH := IHcount (S offset)). clear IHcount.
+f_equal. { f_equal. lia. }
+assert (EqLHS:
+          forall t,
+            (fix var_range' (countdown : nat) : list AST.expr :=
+             match countdown with
+             | 0 => nil
+             | S k => AST.LocalVar (N.of_nat (offset + S count - 1 - k)) :: var_range' k
+             end) t
+              =
+            (fix var_range' (countdown : nat) : list AST.expr :=
+             match countdown with
+             | 0 => nil
+             | S k => AST.LocalVar (N.of_nat (S offset + count - 1 - k)) :: var_range' k
+             end) t).
+{
+  clear IH. intro t.
+  revert offset. induction t. { easy. }
+  intro offset.
+  f_equal. 2:apply IHt.
+  f_equal. f_equal. lia.
+}
+rewrite EqLHS. clear EqLHS.
+assert (EqRHS:
+          forall t,
+            (fix var_range' (countdown : nat) : list AST.expr :=
+             match countdown with
+             | 0 => nil
+             | S k =>
+                 AST.LocalVar (N.of_nat offset + N.pos (Pos.of_succ_nat count) - 1 - N.of_nat k) :: var_range' k
+             end) t
+              =
+            (fix var_range' (countdown : nat) : list AST.expr :=
+             match countdown with
+             | 0 => nil
+             | S k => AST.LocalVar (N.of_nat (S offset) + N.of_nat count - 1 - N.of_nat k) :: var_range' k
+             end) t).
+{
+  clear IH. intro t.
+  revert offset. induction t. { easy. }
+  intro offset.
+  f_equal. 2:apply IHt.
+  f_equal. f_equal. lia.
+}
+rewrite EqRHS. clear EqRHS.
+apply IH.
+Qed.
+
+Lemma var_range_via_nat {C: VyperConfig} (offset count: N):
+  var_range offset count = var_range_nat (N.to_nat offset) (N.to_nat count).
+Proof.
+rewrite var_range_nat_ok.
+now repeat rewrite N2Nat.id.
+Qed.
+
+
+Definition translate_small_stmt {C: VyperConfig}
+                                (B: builtin_names_config)
+                                (declmap: string_map L30.AST.decl)
+                                (ss: L30.AST.small_stmt)
 : string + list L40.AST.stmt
 := let op_err := "an operator in L30 can't possibly occur after the CheckArith pass"%string in
    match ss with
@@ -76,25 +152,37 @@ Definition translate_small_stmt {C: VyperConfig} (B: builtin_names_config) (ss: 
    | L30.AST.Copy dst src =>
       inr ((L40.AST.SmallStmt (L40.AST.Assign dst (L40.AST.LocalVar src))) :: nil)
    | L30.AST.StorageGet dst name =>
-      inr ((L40.AST.SmallStmt
-              (L40.AST.Assign dst
-                (L40.AST.BuiltinCall
-                  (builtin_name_sload B)
-                  (L40.AST.Const (string_hash name) :: nil)))) :: nil)
+      match map_lookup declmap name with
+      | Some (L30.AST.StorageVarDecl _) =>
+          inr ((L40.AST.SmallStmt
+                  (L40.AST.Assign dst
+                    (L40.AST.BuiltinCall
+                      (builtin_name_sload B)
+                      (L40.AST.Const (string_hash name) :: nil)))) :: nil)
+      | _ => inl ("undeclared global variable: " ++ name)%string
+      end
    | L30.AST.StoragePut name src =>
-      inr ((L40.AST.SmallStmt
-              (L40.AST.ExprStmt
-                (L40.AST.BuiltinCall
-                  (builtin_name_sstore B)
-                  (L40.AST.Const (string_hash name) :: L40.AST.LocalVar src :: nil)))) :: nil)
+      match map_lookup declmap name with
+      | Some (L30.AST.StorageVarDecl _) =>
+          inr ((L40.AST.SmallStmt
+                  (L40.AST.ExprStmt
+                    (L40.AST.BuiltinCall
+                      (builtin_name_sstore B)
+                      (L40.AST.Const (string_hash name) :: L40.AST.LocalVar src :: nil)))) :: nil)
+      | _ => inl ("undeclared global variable: " ++ name)%string
+      end
    | L30.AST.UnOp _ _ _ => inl op_err
    | L30.AST.PowConstBase _ _ _ => inl op_err
    | L30.AST.PowConstExp _ _ _ => inl op_err
    | L30.AST.BinOp _ _ _ _ _ => inl op_err
    | L30.AST.PrivateCall dst name args_offset args_count =>
-        inr ((L40.AST.SmallStmt
-               (L40.AST.Assign dst
-                 (L40.AST.PrivateCall name (var_range args_offset args_count)))) :: nil)
+        match map_lookup declmap name with
+        | Some (L30.AST.FunDecl _ _ _) =>
+            inr ((L40.AST.SmallStmt
+                   (L40.AST.Assign dst
+                     (L40.AST.PrivateCall name (var_range args_offset args_count)))) :: nil)
+        | _ => inl ("unable to resolve function: " ++ name)%string
+        end
    | L30.AST.BuiltinCall dst name args_offset args_count =>
         inr ((L40.AST.SmallStmt
                (L40.AST.Assign dst
@@ -107,24 +195,27 @@ Definition translate_small_stmt {C: VyperConfig} (B: builtin_names_config) (ss: 
         inr ((L40.AST.SmallStmt (L40.AST.Raise  (L40.AST.LocalVar var))) :: nil)
    end.
 
-Fixpoint translate_stmt {C: VyperConfig} (B: builtin_names_config) (s: L30.AST.stmt)
+Fixpoint translate_stmt {C: VyperConfig}
+                        (B: builtin_names_config)
+                        (declmap: string_map L30.AST.decl)
+                        (s: L30.AST.stmt)
 {struct s}
 : string + list L40.AST.stmt
 := match s with
-   | L30.AST.SmallStmt ss => translate_small_stmt B ss
+   | L30.AST.SmallStmt ss => translate_small_stmt B declmap ss
    | L30.AST.Semicolon a b =>
-      match translate_stmt B a with
+      match translate_stmt B declmap a with
       | inl err => inl err
-      | inr aa => match translate_stmt B b with
+      | inr aa => match translate_stmt B declmap b with
                   | inl err => inl err
                   | inr bb => inr (aa ++ bb)
                   end
       end
    | L30.AST.IfElseStmt condvar yes no =>
-      match translate_stmt B yes with
+      match translate_stmt B declmap yes with
       | inl err => inl err
       | inr yes' =>
-          match translate_stmt B no with 
+          match translate_stmt B declmap no with 
           | inl err => inl err
           | inr no' =>
               inr (L40.AST.Switch (L40.AST.LocalVar condvar)
@@ -136,31 +227,36 @@ Fixpoint translate_stmt {C: VyperConfig} (B: builtin_names_config) (s: L30.AST.s
       let count_z := Z_of_uint256 count in
       if (count_z =? 0)%Z
         then inl "zero-count loops are not allowed"
-        else match translate_stmt B body with
+        else match translate_stmt B declmap body with
              | inl err => inl err
              | inr body' =>
                   inr
                     (* start_z + count_z - 1 < 2^256
                         <->
-                       start_z < 2^256 - count_z + 1 *)
+                       start_z <= 2^256 - count_z *)
                     (L40.AST.Switch
                       (L40.AST.BuiltinCall
                         (builtin_name_uint256_lt B)
-                          (L40.AST.LocalVar loopvar
-                             ::L40.AST.Const (uint256_of_Z (2 ^ 256 - count_z + 1)%Z)
+                          (L40.AST.Const (uint256_of_Z (2 ^ 256 - count_z)%Z)
+                             :: L40.AST.LocalVar loopvar
                              :: nil))
-                      (L40.AST.Case zero256
+                      ((L40.AST.Case zero256
                         (L40.AST.Block
-                          (L40.AST.SmallStmt
-                            (L40.AST.Abort
-                              (AbortException (uint256_of_Z (Z_of_string "loop range overflows"))))
-                          :: nil)) :: nil)
+                          ((L40.AST.Loop loopvar count
+                            (L40.AST.Block
+                              ((L40.AST.SmallStmt
+                                (L40.AST.Assign loopvar
+                                  (L40.AST.BuiltinCall (builtin_name_uint256_add B)
+                                    (L40.AST.LoopOffset :: L40.AST.LoopCursor :: nil))))
+                                :: body')))
+                            :: nil)))
+                        :: nil)
                       (Some
                         (L40.AST.Block
                           ((L40.AST.SmallStmt
-                            (L40.AST.Assign loopvar
-                              (L40.AST.BuiltinCall (builtin_name_uint256_add B)
-                                (L40.AST.LoopOffset :: L40.AST.LoopCursor :: nil))))
-                          :: body'))) :: nil)
+                            (L40.AST.Abort
+                              (AbortException (uint256_of_Z (Z_of_string "loop range overflows")))))
+                            :: nil)))
+                        :: nil)
              end
    end.
