From30To40/Stmt.v
@@ -1,0 +1,1145 @@
+From Coq Require Import String ZArith NArith Lia PropExtensionality.
+
+
+From Vyper Require Import Config Builtins Calldag Logic2.
+From Vyper.L10 Require Import Base.
+From Vyper.L30 Require AST Callset Interpret.
+From Vyper.L40 Require AST Callset Interpret.
+From Vyper.From30To40 Require Import FunCtx Translate.
+
+(** XXX this is not necessary *)
+Lemma var_range_callset {C: VyperConfig} (args_offset args_count: N):
+  let _ := string_set_impl in
+  FSet.is_empty
+    (L40.Callset.expr_list_callset (var_range args_offset args_count))
+   = true.
+Proof.
+cbn.
+rewrite var_range_via_nat.
+unfold var_range_nat.
+remember (N.to_nat args_count) as n.
+clear Heqn.
+revert args_offset.
+induction n; intros. { cbn. rewrite FSet.is_empty_to_list. apply FSet.empty_to_list. }
+cbn. rewrite FSet.is_empty_true_iff.
+intro x. rewrite FSet.union_ok. rewrite FSet.empty_ok. rewrite Bool.orb_false_l. 
+assert (IH := IHn (N.succ args_offset)). rewrite FSet.is_empty_true_iff in IH.
+assert (R: forall t,
+             (fix var_range' (countdown : nat) : list AST.expr :=
+               match countdown with
+               | 0 => nil
+               | S k => (AST.LocalVar (N.of_nat (N.to_nat args_offset + S n - 1 - k)) :: var_range' k)%list
+               end) t
+            =
+            (fix var_range' (countdown : nat) : list AST.expr :=
+              match countdown with
+              | 0 => nil
+              | S k =>
+                  (AST.LocalVar (N.of_nat (N.to_nat (N.succ args_offset) + n - 1 - k)) :: var_range' k)%list
+              end) t).
+{
+  induction t. { trivial. }
+  f_equal. { f_equal. lia. }
+  apply IHt.
+}
+rewrite R. clear R. apply IH.
+Qed.
+
+(** Interpreting [var_range] always succeeds and results in a view of the local memory
+    that can also be obtained directly by [OpenArray.view].
+ *)
+Lemma interpret_var_range
+          {C: VyperConfig}
+          {smaller_call_depth_bound: nat}
+          (B: builtin_names_config)
+          {cd30: L30.Descend.calldag}
+          {cd40: L40.Descend.calldag}
+          (CalldagOk: translate_calldag B cd30 = inr cd40)
+          (fc30: fun_ctx cd30 (S smaller_call_depth_bound))
+          (FcNotVar: forall x,
+                       fun_decl fc30 <> AST.StorageVarDecl x)
+          (do_call_40: forall
+                (fc': fun_ctx cd40 smaller_call_depth_bound)
+                (world: world_state)
+                (arg_values: list uint256),
+              world_state * expr_result uint256)
+          (builtins: string -> option builtin)
+          (world: world_state)
+          (loc: memory)
+          (loopinfo: list L40.Expr.loop_ctx)
+          (args_offset args_count: N)
+          CallOk:
+      let _ := memory_impl in
+      let fix interpret_expr_list
+                (world0 : world_state) (loc0 : memory) (e : list AST.expr)
+                (CallOk : FSet.is_subset (Callset.expr_list_callset e)
+                            (Callset.decl_callset (cached_translated_decl fc30 B CalldagOk FcNotVar)) =
+                          true) {struct e} : world_state * expr_result (list uint256) :=
+                match e as e' return (e = e' -> world_state * expr_result (list uint256)) with
+                | nil => fun _ : e = nil => (world0, ExprSuccess nil)
+                | (h :: t)%list =>
+                    fun E : e = (h :: t)%list =>
+                    let (world', result_t) :=
+                      interpret_expr_list world0 loc0 t (Callset.callset_descend_tail E CallOk) in
+                    match result_t with
+                    | ExprSuccess values_t =>
+                        let (world'', result_h) :=
+                          L40.Expr.interpret_expr eq_refl (translate_fun_ctx fc30 B CalldagOk FcNotVar)
+                            do_call_40 builtins world' loc0 loopinfo h
+                            (Callset.callset_descend_head E CallOk) in
+                        (world'',
+                        match result_h with
+                        | ExprSuccess value_h => ExprSuccess (value_h :: values_t)%list
+                        | ExprAbort ab => ExprAbort ab
+                        end)
+                    | ExprAbort ab => (world', ExprAbort ab)
+                    end
+                end eq_refl
+      in
+        interpret_expr_list world loc 
+                            (var_range args_offset args_count)
+                            CallOk
+         =
+        (world, ExprSuccess (OpenArray.view loc args_offset args_count)).
+Proof.
+intros.
+revert CallOk. rewrite var_range_via_nat. intro CallOk.
+assert (V' := OpenArray.view_ok loc args_offset args_count).
+assert (L := OpenArray.view_len loc args_offset args_count).
+remember (OpenArray.view loc args_offset args_count) as v. clear Heqv.
+(* a variant of V' with nats: *)
+assert (V:
+  forall k: nat, (k < (N.to_nat args_count)%N) -> 
+    List.nth_error v k = Some (OpenArray.get loc (args_offset + (N.of_nat k)))).
+{
+  intros k H.
+  rewrite<- (V' (N.of_nat k)). { now rewrite Nat2N.id. }
+  rewrite<- N.compare_lt_iff.
+  rewrite<- (N2Nat.id args_count).
+  rewrite<- Nat2N.inj_compare.
+  rewrite Nat.compare_lt_iff.
+  exact H.
+}
+clear V'.
+rewrite<- L in V.
+remember (N.to_nat args_count) as n.
+revert CallOk.
+replace args_count with (N.of_nat n) in *. 2:{ subst. apply N2Nat.id. }
+clear args_count Heqn.
+intros. unfold var_range_nat.
+
+revert args_offset v V L CallOk.
+enough (T: forall  (t: nat) (args_offset: N) (v: list uint256),
+            (forall k : nat,
+               k < Datatypes.length v ->
+                 List.nth_error v k
+                  =
+                 Some (OpenArray.get loc (args_offset + N.of_nat (k + n - t)))) ->
+            Datatypes.length v = t ->
+            t <= n ->
+            forall CallOk,
+              interpret_expr_list world loc
+                ((fix var_range' (countdown : nat) : list AST.expr :=
+                    match countdown with
+                    | 0 => nil
+                    | S k => (AST.LocalVar (N.of_nat (N.to_nat args_offset + n - 1 - k)) 
+                             :: var_range' k)%list
+                    end) t) CallOk = (world, ExprSuccess v)).
+{
+  intros.
+  assert (W: forall k: nat,
+               k < Datatypes.length v ->
+               List.nth_error v k = Some (OpenArray.get loc (args_offset + N.of_nat (k + n - n)))).
+  { intros. rewrite Nat.add_sub. now apply V. }
+  apply (T n args_offset v W L (Nat.le_refl n)).
+}
+induction t. { intros. cbn. now destruct v. }
+intros args_offset v V' L' Bound CallOk. cbn.
+destruct v as [|h]. { discriminate. }
+assert (L: Datatypes.length v = t) by now inversion L'.
+assert (V: forall k: nat,
+             k < Datatypes.length v ->
+             List.nth_error v k = Some (OpenArray.get loc (args_offset + N.of_nat (k + n - t)))).
+{
+  intro k. assert (W := V' (S k)). cbn in W.
+  intro Bk. rewrite W by lia.
+  f_equal.
+}
+assert (Bt: t <= n) by lia.
+rewrite (IHt args_offset v V L Bt).
+repeat f_equal.
+assert (W := V' 0 (Nat.lt_0_succ _)).
+cbn in W.
+inversion W. subst. f_equal. lia.
+Qed.
+
+Lemma interpret_translated_small_stmt
+    {C: VyperConfig}
+    {bigger_call_depth_bound smaller_call_depth_bound: nat}
+    (B: builtin_names_config)
+    (Ebound: bigger_call_depth_bound = S smaller_call_depth_bound)
+    {cd30: L30.Descend.calldag}
+    {cd40: L40.Descend.calldag}
+    (CalldagOk: translate_calldag B cd30 = inr cd40)
+    (fc30: fun_ctx cd30 bigger_call_depth_bound)
+    (FcNotVar: forall x,
+                 fun_decl fc30 <> AST.StorageVarDecl x)
+    {do_call_30: forall
+          (fc': fun_ctx cd30 smaller_call_depth_bound)
+          (world: world_state)
+          (arg_values: list uint256),
+        world_state * expr_result uint256}
+    {do_call_40: forall
+          (fc': fun_ctx cd40 smaller_call_depth_bound)
+          (world: world_state)
+          (arg_values: list uint256),
+        world_state * expr_result uint256}
+    (DoCallOk:
+       forall fc'
+              (NotVar: forall x, fun_decl fc' <> AST.StorageVarDecl x)
+              world arg_values,
+         do_call_40 (translate_fun_ctx fc' B CalldagOk NotVar) world arg_values
+          =
+         do_call_30 fc' world arg_values)
+    {ss30: L30.AST.small_stmt}
+    {l40: list L40.AST.stmt}
+    (ok: translate_small_stmt B (cd_decls cd30) ss30 = inr l40)
+    (builtins: string -> option builtin)
+    (SloadOk: BuiltinsSupportSload B builtins)
+    (SstoreOk: BuiltinsSupportSstore B builtins)
+    (world: world_state)
+    (loc: memory)
+    (CallOk30: let _ := string_set_impl in 
+               FSet.is_subset (L30.Callset.small_stmt_callset ss30)
+                              (L30.Callset.decl_callset (fun_decl fc30))
+               = true)
+    (CallOk40: let _ := string_set_impl in 
+               FSet.is_subset (L40.Callset.stmt_list_callset l40)
+                              (L40.Callset.decl_callset
+                                (fun_decl
+                                  (translate_fun_ctx fc30 B CalldagOk FcNotVar)))
+               = true)
+    (loopinfo: list L40.Expr.loop_ctx):
+  L30.Stmt.interpret_small_stmt Ebound fc30 do_call_30 builtins world loc ss30 CallOk30
+   =
+  L40.Stmt.interpret_block Ebound (translate_fun_ctx fc30 B CalldagOk FcNotVar)
+                                  do_call_40 builtins world loc loopinfo
+                                  (L40.AST.Block l40) CallOk40.
+Proof.
+destruct ss30; cbn in ok; try discriminate; inversion ok; subst; try easy.
+{ (* sload *)
+  unfold BuiltinsSupportSload in SloadOk. cbn.
+  unfold cd_declmap. unfold map_lookup in *.
+  destruct (Map.lookup (cd_decls cd30) name) as [d|]. 2:discriminate.
+  destruct d. 2:discriminate.
+  cbn.
+  remember (builtin_name_sload B) as sload_name.
+  cbn.
+  remember (builtins sload_name) as sload_builtin.
+  destruct sload_builtin as [(sload_arity, sload)|]. 2:contradiction.
+  destruct sload_arity. { contradiction. }
+  destruct sload_arity. 2: contradiction.
+  inversion ok; subst l40. cbn.
+  assert (K := SloadOk world name).
+  remember (sload world (string_hash name)) as sload_result.
+  destruct sload_result as (world', result).
+  destruct result. 2:contradiction.
+  destruct K as (W, V).
+  rewrite<- Heqsload_builtin. cbn.
+  subst world' value.
+  now rewrite<- Heqsload_result.
+}
+{ (* sstore *)
+  unfold BuiltinsSupportSstore in SstoreOk. cbn.
+  unfold cd_declmap. unfold map_lookup in *.
+  destruct (Map.lookup (cd_decls cd30) name) as [d|]. 2:discriminate.
+  destruct d. 2:discriminate.
+  cbn.
+  remember (builtin_name_sstore B) as sstore_name.
+  cbn.
+  remember (builtins sstore_name) as sstore_builtin.
+  destruct sstore_builtin as [(sstore_arity, sstore)|]. 2:contradiction.
+  destruct sstore_arity. { contradiction. }
+  destruct sstore_arity. { contradiction. }
+  destruct sstore_arity. 2: contradiction.
+  inversion ok; subst l40. cbn.
+  assert (K := let _ := memory_impl in SstoreOk world name (OpenArray.get loc src)).
+  remember (sstore world (string_hash name) _) as sstore_result.
+  destruct sstore_result as (world', result).
+  destruct result. 2:contradiction.
+  rewrite<- Heqsstore_builtin. cbn.
+  subst.
+  now rewrite<- Heqsstore_result.
+}
+{ (* PrivateCall *)
+  remember (map_lookup (cd_decls cd30) name) as lookup_result.
+  destruct lookup_result as [d|]. 2:discriminate.
+  destruct d. 1:discriminate.
+  unfold L30.Descend.fun_ctx_descend.
+  unfold L40.Descend.fun_ctx_descend.
+  assert (D := translate_fun_ctx_declmap B CalldagOk name).
+  inversion ok; subst; clear ok.
+  unfold Translate.var_range in *. cbn.
+  remember (Callset.callset_descend_assign_rhs eq_refl
+              (Callset.callset_descend_small_stmt eq_refl
+                 (Callset.callset_descend_stmts_head eq_refl
+                    (Callset.callset_descend_block eq_refl _))))
+    as CallOkRHS40.
+  unfold L30.Descend.fun_ctx_descend.
+  unfold L40.Descend.fun_ctx_descend.
+  unfold cd_declmap in *. unfold map_lookup in *.
+  remember (fix interpret_expr_list
+                  (world0 : world_state) (loc0 : memory) (e : list AST.expr)
+                  (CallOk : FSet.is_subset (Callset.expr_list_callset e)
+                              (Callset.decl_callset (cached_translated_decl fc30 B CalldagOk FcNotVar)) =
+                            true) {struct e} : world_state * expr_result (list uint256) := _)
+    as interpret_expr_list.
+  remember (fun d (Edecl : Map.lookup (cd_decls cd30) name = Some d) =>
+      L30.Descend.fun_ctx_descend_inner fc30 CallOk30
+        eq_refl eq_refl Edecl)
+    as good_branch_30.
+  remember (fun d (Edecl : Map.lookup (cd_decls cd40) name = Some d) =>
+              Descend.fun_ctx_descend_inner (translate_fun_ctx fc30 B CalldagOk FcNotVar) CallOkRHS40
+                                            eq_refl eq_refl Edecl)
+    as good_branch_40.
+  remember (fix var_range' (countdown : nat) : list AST.expr :=
+               match countdown with
+               | 0 => nil
+               | S k =>
+                   (AST.LocalVar (args_offset + args_count - 1 - N.of_nat k) :: var_range' k)%list
+               end)
+    as var_range.
+  (* Coq has problems typing this in a bigger expression *)
+  remember (fun y (Ey: Map.lookup (cd_decls cd40) name = Some y) =>
+                         match good_branch_40 y Ey with
+                         | Some new_fc =>
+                            let (world', result_args) :=
+                              interpret_expr_list world loc (var_range (N.to_nat args_count))
+                                (Callset.callset_descend_args eq_refl CallOkRHS40) in
+                            match result_args with
+                            | ExprSuccess arg_values => do_call_40 new_fc world' arg_values
+                            | ExprAbort ab => (world', ExprAbort ab)
+                            end
+                         | None => (world, expr_error "can't resolve function name")
+                         end)
+    as compute40.
+  enough (W:
+    forall x (Ex: Map.lookup (cd_decls cd30) name = Some x)
+           y (Ey: Map.lookup (cd_decls cd40) name = Some y),
+      let _ := memory_impl in
+      match good_branch_30 x Ex with
+      | Some new_fc =>
+          let (world', call_result) := do_call_30 new_fc world (OpenArray.view loc args_offset args_count) in
+          match call_result with
+          | ExprSuccess result => (world', OpenArray.put loc dst result, StmtSuccess)
+          | ExprAbort ab => (world', loc, StmtAbort ab)
+          end
+      | None => (world, loc, stmt_error "can't resolve function name")
+      end =
+      match
+        (let '(world', result) := compute40 y Ey in
+         match result with
+         | ExprSuccess value => (world', OpenArray.put loc dst value, StmtSuccess)
+         | ExprAbort ab => (world', loc, StmtAbort ab)
+         end)
+      return world_state * memory * stmt_result uint256
+      with
+      | (world', loc', StmtSuccess) => (world', loc', StmtSuccess)
+      | (world', loc', StmtAbort _ as result) | (world', loc', StmtReturnFromFunction _ as result) =>
+          (world', loc', result)
+      end).
+  {
+    clear Heqgood_branch_30.
+    clear Heqgood_branch_40.
+    destruct (Map.lookup (cd_decls cd30) name) as [d30|],
+             (Map.lookup (cd_decls cd40) name) as [d40|]; cbn;
+      try destruct d30; try destruct d40; try easy.
+    subst compute40.
+    apply W.
+  }
+  (* following InnerOk from From20To30/Expr.v *)
+  intros x Ex y Ey. cbn.
+  subst good_branch_30 compute40 good_branch_40.
+  cbn.
+  rewrite Ex in D. rewrite Ey in D.
+  remember (match
+                       match
+                         Descend.fun_ctx_descend_inner (translate_fun_ctx fc30 B CalldagOk FcNotVar) CallOkRHS40 eq_refl eq_refl Ey
+                       with
+                       | Some new_fc =>
+                           let (world', result_args) :=
+                             interpret_expr_list world loc (var_range (N.to_nat args_count))
+                               (Callset.callset_descend_args eq_refl CallOkRHS40) in
+                           match result_args with
+                           | ExprSuccess arg_values => do_call_40 new_fc world' arg_values
+                           | ExprAbort ab => (world', ExprAbort ab)
+                           end
+                       | None => (world, expr_error "can't resolve function name")
+                       end
+                     with
+                     | (world', ExprSuccess value) => (world', OpenArray.put loc dst value, StmtSuccess)
+                     | (world', ExprAbort ab) => (world', loc, StmtAbort ab)
+                     end) as rhs.
+  (* this silliness is happening because we translate from
+     stmt_result to expr_result and back *)
+  replace ((let (p, result) := rhs in
+             let (world', loc') := p in
+             match result with
+             | StmtSuccess => (world', loc', StmtSuccess)
+             | _ => (world', loc', result)
+             end))
+    with rhs
+    by now destruct rhs as ((world', loc'), result), result.
+  subst rhs.
+  unfold L30.Descend.fun_ctx_descend_inner.
+  unfold L40.Descend.fun_ctx_descend_inner.
+  remember (fun (depth: nat) (Edepth: cd_depthmap cd30 name = Some depth) =>
+      Some
+        {|
+          fun_name := name;
+          fun_depth := depth;
+          fun_depth_ok := Edepth;
+          fun_decl := x;
+          fun_decl_ok := Ex;
+          fun_bound_ok := _
+        |})
+    as some_branch_l.
+  remember (fun Edepth : cd_depthmap cd30 name = None =>
+              False_rect (option (fun_ctx cd30 smaller_call_depth_bound))
+                         (L30.Descend.fun_ctx_descend_helper Ex Edepth))
+    as none_branch_l.
+  remember (fun (depth: nat) (Edepth: cd_depthmap cd40 name = Some depth) =>
+    Some
+      {|
+        fun_name := name;
+        fun_depth := depth;
+        fun_depth_ok := Edepth;
+        fun_decl := y;
+        fun_decl_ok := Ey;
+        fun_bound_ok := _
+      |})
+    as some_branch_r.
+  remember (fun Edepth : cd_depthmap cd40 name = None =>
+                False_rect (option (fun_ctx cd40 smaller_call_depth_bound))
+                  (L40.Descend.fun_ctx_descend_helper Ey Edepth))
+    as none_branch_r.
+  assert (NoneOkL: forall (Edepth: cd_depthmap cd30 name = None),
+                     none_branch_l Edepth = None).
+  { intro. exfalso. exact (L30.Descend.fun_ctx_descend_helper Ex Edepth). }
+  assert (NoneOkR: forall (Edepth: cd_depthmap cd40 name = None),
+                     none_branch_r Edepth = None).
+  { intro. exfalso. exact (L40.Descend.fun_ctx_descend_helper Ey Edepth). }
+  clear Heqnone_branch_l Heqnone_branch_r.
+  enough (SomeBranchOk:
+      forall (depth: nat)
+             (Edepth30: cd_depthmap cd30 name = Some depth)
+             (Edepth40: cd_depthmap cd40 name = Some depth),
+       let _ := memory_impl in
+        match some_branch_l depth Edepth30
+        return (world_state * memory * stmt_result uint256)
+        with
+        | Some new_fc =>
+            let (world', call_result) := do_call_30 new_fc world (OpenArray.view loc args_offset args_count) in
+            match call_result with
+            | ExprSuccess result => (world', OpenArray.put loc dst result, StmtSuccess)
+            | ExprAbort ab => (world', loc, StmtAbort ab)
+            end
+        | None => (world, loc, stmt_error "can't resolve function name")
+        end =
+        let (world', e) :=
+           match some_branch_r depth Edepth40 with
+           | Some new_fc =>
+               let (world', result_args) :=
+                 interpret_expr_list world loc (var_range (N.to_nat args_count))
+                   (Callset.callset_descend_args eq_refl CallOkRHS40) in
+               match result_args with
+               | ExprSuccess arg_values => do_call_40 new_fc world' arg_values
+               | ExprAbort ab => (world', ExprAbort ab)
+               end
+           | None => (world, expr_error "can't resolve function name")
+           end in
+         match e with
+         | ExprSuccess value => (world', OpenArray.put loc dst value, StmtSuccess)
+         | ExprAbort ab => (world', loc, StmtAbort ab)
+         end).
+  {
+    revert none_branch_l none_branch_r NoneOkL NoneOkR.
+    clear Heqsome_branch_l Heqsome_branch_r
+          CallOk30 CallOk40 HeqCallOkRHS40 Ex Ey x y D DoCallOk.
+    revert some_branch_l some_branch_r SomeBranchOk.
+    rewrite (translate_fun_ctx_depthmap B CalldagOk name).
+    destruct (cd_depthmap cd30 name); intros. { apply SomeBranchOk. }
+    rewrite (NoneOkL eq_refl).
+    rewrite (NoneOkR eq_refl).
+    trivial.
+  }
+  intros. subst some_branch_l some_branch_r.
+  unfold translate_fun_ctx. cbn.
+  subst interpret_expr_list var_range.
+  assert (R := interpret_var_range B CalldagOk fc30 FcNotVar do_call_40 builtins world loc loopinfo
+                                   args_offset args_count
+                                   (Callset.callset_descend_args eq_refl CallOkRHS40)).
+  unfold var_range. unfold var_range in R. rewrite R. clear R.
+  assert (FcNotVar': forall str: string,
+                       fun_decl
+                         {|
+                           fun_name := name;
+                           fun_depth := depth;
+                           fun_depth_ok := Edepth30;
+                           fun_decl := x;
+                           fun_decl_ok := Ex;
+                           fun_bound_ok := L30.Descend.call_descend' fc30 CallOk30 eq_refl eq_refl Ex Edepth30
+                         |} <> AST.StorageVarDecl str).
+  {
+    cbn. intros str H. subst x.
+    destruct y as (y_name, y_nargs, y_body).
+    now destruct y_body.
+  }
+  rewrite<- (DoCallOk _ FcNotVar').
+  remember (L30.Descend.call_descend' _ _ _ _ _ _) as DescendOk30.
+  remember (L40.Descend.call_descend' _ _ _ _ _ _) as DescendOk40.
+  assert (EDescend: DescendOk30 = DescendOk40)
+    by apply proof_irrelevance.
+  clear HeqDescendOk30 HeqDescendOk40.
+  subst DescendOk40.
+  enough (E: translate_fun_ctx
+                {|
+                  fun_name := name;
+                  fun_depth := depth;
+                  fun_depth_ok := Edepth30;
+                  fun_decl := x;
+                  fun_decl_ok := Ex;
+                  fun_bound_ok := DescendOk30
+                |} B CalldagOk FcNotVar'
+               =
+               {|
+                 fun_name := name;
+                 fun_depth := depth;
+                 fun_depth_ok := Edepth40;
+                 fun_decl := y;
+                 fun_decl_ok := Ey;
+                 fun_bound_ok := DescendOk30
+               |})
+    by now rewrite E.
+  unfold translate_fun_ctx. cbn.
+  enough (E: y = cached_translated_decl
+              {|
+                fun_name := name;
+                fun_depth := depth;
+                fun_depth_ok := Edepth30;
+                fun_decl := x;
+                fun_decl_ok := Ex;
+                fun_bound_ok := DescendOk30
+              |} B CalldagOk FcNotVar').
+  {
+    subst.
+    assert (R: eq_trans (translate_fun_ctx_depthmap B CalldagOk name) Edepth30 = Edepth40)
+      by apply proof_irrelevance. rewrite R. clear R.
+    assert (R: Ey = FunCtx.translate_fun_ctx_decl_ok
+                {|
+                  fun_name := name;
+                  fun_depth := depth;
+                  fun_depth_ok := Edepth30;
+                  fun_decl := x;
+                  fun_decl_ok := Ex;
+                  fun_bound_ok := DescendOk30
+                |} B CalldagOk FcNotVar')
+      by apply proof_irrelevance.
+    now subst.
+  }
+  unfold cached_translated_decl. cbn.
+  unfold cd_declmap.
+  remember (fun E : Map.lookup (cd_decls cd40) name = None =>
+              False_rect AST.decl _) as none_branch. clear Heqnone_branch.
+  destruct (Map.lookup (cd_decls cd40) name).
+  { now inversion Ey. }
+  discriminate.
+}
+(* builtin *)
+cbn.
+rewrite interpret_var_range.
+destruct (builtins name) as [(arity, builtin)|]. 2:easy.
+remember (fun Earity : (arity =? Datatypes.length (OpenArray.view loc args_offset args_count)) = true =>
+            let '(world', call_result) :=
+              call_builtin (OpenArray.view loc args_offset args_count) Earity (builtin world) in
+            match call_result return world_state * memory * stmt_result uint256 with
+            | ExprSuccess result => (world', OpenArray.put loc dst result, StmtSuccess)
+            | ExprAbort ab => (world', loc, StmtAbort ab)
+            end)
+  as good_branch_l.
+remember (fun Earity : (arity =? Datatypes.length (OpenArray.view loc args_offset args_count)) = true =>
+            call_builtin (OpenArray.view loc args_offset args_count) Earity (builtin world))
+  as good_branch_r.
+enough (W: forall (Earity: arity =? Datatypes.length (OpenArray.view loc args_offset args_count) = true),
+             let _ := memory_impl in
+             good_branch_l Earity =
+              match
+                (let '(world', result) := good_branch_r Earity in
+                 match result return world_state * memory * stmt_result uint256 with
+                 | ExprSuccess value => (world', OpenArray.put loc dst value, StmtSuccess)
+                 | ExprAbort ab => (world', loc, StmtAbort ab)
+                 end)
+              with
+              | (world', loc', StmtSuccess) => (world', loc', StmtSuccess)
+              | (world', loc', StmtAbort _ as result) | (world', loc', StmtReturnFromFunction _ as result) =>
+                  (world', loc', result)
+              end).
+{
+  clear Heqgood_branch_l. clear Heqgood_branch_r.
+  now destruct (arity =? Datatypes.length (OpenArray.view loc args_offset args_count)).
+}
+intro Earity. cbn. subst.
+destruct (call_builtin (OpenArray.view loc args_offset args_count) Earity (builtin world))
+  as (new_world, result).
+now destruct result.
+Qed.
+
+(******************************************************************************************)
+
+Lemma interpret_translated_stmt
+    {C: VyperConfig}
+    {bigger_call_depth_bound smaller_call_depth_bound: nat}
+    (B: builtin_names_config)
+    (Ebound: bigger_call_depth_bound = S smaller_call_depth_bound)
+    {cd30: L30.Descend.calldag}
+    {cd40: L40.Descend.calldag}
+    (CalldagOk: translate_calldag B cd30 = inr cd40)
+    (fc30: fun_ctx cd30 bigger_call_depth_bound)
+    (FcNotVar: forall x,
+                 fun_decl fc30 <> AST.StorageVarDecl x)
+    {do_call_30: forall
+          (fc': fun_ctx cd30 smaller_call_depth_bound)
+          (world: world_state)
+          (arg_values: list uint256),
+        world_state * expr_result uint256}
+    {do_call_40: forall
+          (fc': fun_ctx cd40 smaller_call_depth_bound)
+          (world: world_state)
+          (arg_values: list uint256),
+        world_state * expr_result uint256}
+    (DoCallOk:
+       forall fc'
+              (NotVar: forall x, fun_decl fc' <> AST.StorageVarDecl x)
+              world arg_values,
+         do_call_40 (translate_fun_ctx fc' B CalldagOk NotVar) world arg_values
+          =
+         do_call_30 fc' world arg_values)
+    {s30: L30.AST.stmt}
+    {l40: list L40.AST.stmt}
+    (ok: translate_stmt B (cd_decls cd30) s30 = inr l40)
+    (builtins: string -> option builtin)
+    (SloadOk: BuiltinsSupportSload B builtins)
+    (SstoreOk: BuiltinsSupportSstore B builtins)
+    (BuiltinsOk: BuiltinsSupportUInt256 B builtins) (* because we need lt() in the loop *)
+    (world: world_state)
+    (loc: memory)
+    (CallOk30: let _ := string_set_impl in 
+               FSet.is_subset (L30.Callset.stmt_callset s30)
+                              (L30.Callset.decl_callset (fun_decl fc30))
+               = true)
+    (CallOk40: let _ := string_set_impl in 
+               FSet.is_subset (L40.Callset.stmt_list_callset l40)
+                              (L40.Callset.decl_callset
+                                (fun_decl
+                                  (translate_fun_ctx fc30 B CalldagOk FcNotVar)))
+               = true)
+    (loopinfo: list L40.Expr.loop_ctx):
+  L30.Stmt.interpret_stmt Ebound fc30 do_call_30 builtins world loc s30 CallOk30
+   =
+  L40.Stmt.interpret_block Ebound (translate_fun_ctx fc30 B CalldagOk FcNotVar)
+                                  do_call_40 builtins world loc loopinfo
+                                  (L40.AST.Block l40) CallOk40.
+Proof.
+revert l40 ok world loc CallOk30 CallOk40 loopinfo. induction s30; intros.
+{ (* small *)
+  apply (interpret_translated_small_stmt B Ebound CalldagOk fc30 FcNotVar DoCallOk
+                                         ok builtins SloadOk SstoreOk).
+}
+{ (* if *)
+  match goal with
+  |- ?l = ?r => remember r as rhs
+  end.
+  cbn. cbn in ok.
+  remember (translate_stmt B (cd_decls cd30) s30_1) as l40_1.
+  destruct l40_1 as [|l40_1]. { discriminate. } symmetry in Heql40_1.
+  remember (translate_stmt B (cd_decls cd30) s30_2) as l40_2.
+  destruct l40_2 as [|l40_2]. { discriminate. } symmetry in Heql40_2.
+  assert (IHs30_1' := IHs30_1 l40_1 eq_refl). clear IHs30_1. rename IHs30_1' into IHs30_1.
+  assert (IHs30_2' := IHs30_2 l40_2 eq_refl). clear IHs30_2. rename IHs30_2' into IHs30_2.
+  inversion ok; subst l40; clear ok.
+
+  remember (Z_of_uint256 (OpenArray.get loc cond_src) =? 0)%Z as cond_is_0.
+  destruct cond_is_0; subst; cbn;
+    replace (Z_of_uint256 zero256) with 0%Z by (unfold zero256; now rewrite uint256_ok);
+    rewrite<- Heqcond_is_0.
+  {
+    assert (CallOk40' := (@Callset.callset_descend_block C l40_2 (@AST.Block C l40_2)
+         (@Callset.decl_callset C
+            (@cached_translated_decl C (S smaller_call_depth_bound) cd30 fc30 cd40 B CalldagOk FcNotVar))
+         (@eq_refl (@AST.block C) (@AST.Block C l40_2))
+         (@Callset.callset_descend_cases_head C (@AST.Case C (@zero256 C) (@AST.Block C l40_2))
+            (@nil (@AST.case C)) (@AST.Case C (@zero256 C) (@AST.Block C l40_2) :: @nil (@AST.case C))
+            (@Callset.decl_callset C
+               (@cached_translated_decl C (S smaller_call_depth_bound) cd30 fc30 cd40 B CalldagOk FcNotVar))
+            (@eq_refl (list (@AST.case C))
+               (@AST.Case C (@zero256 C) (@AST.Block C l40_2) :: @nil (@AST.case C))%list)
+            (@Callset.callset_descend_cases C
+               (@AST.Switch C (@AST.LocalVar C cond_src)
+                  (@AST.Case C (@zero256 C) (@AST.Block C l40_2) :: @nil (@AST.case C))
+                  (@Some (@AST.block C) (@AST.Block C l40_1))) (@AST.LocalVar C cond_src)
+               (@AST.Case C (@zero256 C) (@AST.Block C l40_2) :: @nil (@AST.case C))
+               (@Some (@AST.block C) (@AST.Block C l40_1))
+               (@Callset.decl_callset C
+                  (@cached_translated_decl C (S smaller_call_depth_bound) cd30 fc30 cd40 B CalldagOk
+                     FcNotVar))
+               (@eq_refl (@AST.stmt C)
+                  (@AST.Switch C (@AST.LocalVar C cond_src)
+                     (@AST.Case C (@zero256 C) (@AST.Block C l40_2) :: @nil (@AST.case C))
+                     (@Some (@AST.block C) (@AST.Block C l40_1))))
+               (@Callset.callset_descend_stmts_head C
+                  (@AST.Switch C (@AST.LocalVar C cond_src)
+                     (@AST.Case C (@zero256 C) (@AST.Block C l40_2) :: @nil (@AST.case C))
+                     (@Some (@AST.block C) (@AST.Block C l40_1))) (@nil (@AST.stmt C))
+                  (@AST.Switch C (@AST.LocalVar C cond_src)
+                     (@AST.Case C (@zero256 C) (@AST.Block C l40_2) :: @nil (@AST.case C))
+                     (@Some (@AST.block C) (@AST.Block C l40_1)) :: @nil (@AST.stmt C))
+                  (@Callset.decl_callset C
+                     (@cached_translated_decl C (S smaller_call_depth_bound) cd30 fc30 cd40 B CalldagOk
+                        FcNotVar))
+                  (@eq_refl (list (@AST.stmt C))
+                     (@AST.Switch C (@AST.LocalVar C cond_src)
+                        (@AST.Case C (@zero256 C) (@AST.Block C l40_2) :: @nil (@AST.case C))
+                        (@Some (@AST.block C) (@AST.Block C l40_1)) :: @nil (@AST.stmt C))%list)
+                  (@Callset.callset_descend_block C
+                     (@AST.Switch C (@AST.LocalVar C cond_src)
+                        (@AST.Case C (@zero256 C) (@AST.Block C l40_2) :: @nil (@AST.case C))
+                        (@Some (@AST.block C) (@AST.Block C l40_1)) :: @nil (@AST.stmt C))
+                     (@AST.Block C
+                        (@AST.Switch C (@AST.LocalVar C cond_src)
+                           (@AST.Case C (@zero256 C) (@AST.Block C l40_2) :: @nil (@AST.case C))
+                           (@Some (@AST.block C) (@AST.Block C l40_1)) :: @nil (@AST.stmt C)))
+                     (@Callset.decl_callset C
+                        (@cached_translated_decl C (S smaller_call_depth_bound) cd30 fc30 cd40 B CalldagOk
+                           FcNotVar))
+                     (@eq_refl (@AST.block C)
+                        (@AST.Block C
+                           (@AST.Switch C (@AST.LocalVar C cond_src)
+                              (@AST.Case C (@zero256 C) (@AST.Block C l40_2) :: @nil (@AST.case C))
+                              (@Some (@AST.block C) (@AST.Block C l40_1)) :: @nil (@AST.stmt C))))
+                     CallOk40)))))).
+    rewrite IHs30_2 with (CallOk40 := CallOk40') (loopinfo := loopinfo).
+    cbn.
+    assert (X: forall x: world_state * memory * stmt_result uint256,
+              match x with
+              | (world', loc', StmtSuccess) => (world', loc', StmtSuccess)
+              | (world', loc', StmtAbort _ as result) | (world', loc', StmtReturnFromFunction _ as result) => (world', loc', result)
+              end = x).
+    {
+      intro x. destruct x as ((world', loc'), result). now destruct result.
+    }
+    rewrite X. clear X. f_equal. apply proof_irrelevance.
+  }
+  assert (CallOk40' := (@Callset.callset_descend_block C l40_1 (@AST.Block C l40_1)
+       (@Callset.decl_callset C
+          (@cached_translated_decl C (S smaller_call_depth_bound) cd30 fc30 cd40 B CalldagOk FcNotVar))
+       (@eq_refl (@AST.block C) (@AST.Block C l40_1))
+       (@Callset.callset_descend_cases_default C
+          (@AST.Switch C (@AST.LocalVar C cond_src) (@AST.Case C (@zero256 C) (@AST.Block C l40_2) :: @nil (@AST.case C))
+             (@Some (@AST.block C) (@AST.Block C l40_1))) (@AST.LocalVar C cond_src)
+          (@AST.Case C (@zero256 C) (@AST.Block C l40_2) :: @nil (@AST.case C)) (@AST.Block C l40_1)
+          (@Callset.decl_callset C
+             (@cached_translated_decl C (S smaller_call_depth_bound) cd30 fc30 cd40 B CalldagOk FcNotVar))
+          (@eq_refl (@AST.stmt C)
+             (@AST.Switch C (@AST.LocalVar C cond_src)
+                (@AST.Case C (@zero256 C) (@AST.Block C l40_2) :: @nil (@AST.case C))
+                (@Some (@AST.block C) (@AST.Block C l40_1))))
+          (@Callset.callset_descend_stmts_head C
+             (@AST.Switch C (@AST.LocalVar C cond_src)
+                (@AST.Case C (@zero256 C) (@AST.Block C l40_2) :: @nil (@AST.case C))
+                (@Some (@AST.block C) (@AST.Block C l40_1))) (@nil (@AST.stmt C))
+             (@AST.Switch C (@AST.LocalVar C cond_src)
+                (@AST.Case C (@zero256 C) (@AST.Block C l40_2) :: @nil (@AST.case C))
+                (@Some (@AST.block C) (@AST.Block C l40_1)) :: @nil (@AST.stmt C))
+             (@Callset.decl_callset C
+                (@cached_translated_decl C (S smaller_call_depth_bound) cd30 fc30 cd40 B CalldagOk FcNotVar))
+             (@eq_refl (list (@AST.stmt C))
+                (@AST.Switch C (@AST.LocalVar C cond_src)
+                   (@AST.Case C (@zero256 C) (@AST.Block C l40_2) :: @nil (@AST.case C))
+                   (@Some (@AST.block C) (@AST.Block C l40_1)) :: @nil (@AST.stmt C))%list)
+             (@Callset.callset_descend_block C
+                (@AST.Switch C (@AST.LocalVar C cond_src)
+                   (@AST.Case C (@zero256 C) (@AST.Block C l40_2) :: @nil (@AST.case C))
+                   (@Some (@AST.block C) (@AST.Block C l40_1)) :: @nil (@AST.stmt C))
+                (@AST.Block C
+                   (@AST.Switch C (@AST.LocalVar C cond_src)
+                      (@AST.Case C (@zero256 C) (@AST.Block C l40_2) :: @nil (@AST.case C))
+                      (@Some (@AST.block C) (@AST.Block C l40_1)) :: @nil (@AST.stmt C)))
+                (@Callset.decl_callset C
+                   (@cached_translated_decl C (S smaller_call_depth_bound) cd30 fc30 cd40 B CalldagOk FcNotVar))
+                (@eq_refl (@AST.block C)
+                   (@AST.Block C
+                      (@AST.Switch C (@AST.LocalVar C cond_src)
+                         (@AST.Case C (@zero256 C) (@AST.Block C l40_2) :: @nil (@AST.case C))
+                         (@Some (@AST.block C) (@AST.Block C l40_1)) :: @nil (@AST.stmt C)))) CallOk40))))).
+  rewrite IHs30_1 with (CallOk40 := CallOk40') (loopinfo := loopinfo).
+  cbn.
+  (* XXX dup with the previous branch *)
+  assert (X: forall x: world_state * memory * stmt_result uint256,
+            match x with
+            | (world', loc', StmtSuccess) => (world', loc', StmtSuccess)
+            | (world', loc', StmtAbort _ as result) | (world', loc', StmtReturnFromFunction _ as result) => (world', loc', result)
+            end = x).
+  {
+    intro x. destruct x as ((world', loc'), result). now destruct result.
+  }
+  rewrite X. clear X. f_equal. apply proof_irrelevance.
+}
+2:{ (* Semicolon *)
+  cbn. cbn in ok.
+  remember (fix interpret_stmt_list
+   (world0 : world_state) (loc0 : memory) (loops : list Expr.loop_ctx) (l : list AST.stmt)
+   (Ok : FSet.is_subset (Callset.stmt_list_callset l)
+           (Callset.decl_callset (cached_translated_decl fc30 B CalldagOk FcNotVar)) = true) {struct l} :
+     world_state * memory * stmt_result uint256 := _) as interpret_stmt_list.
+  remember (translate_stmt B (cd_decls cd30) s30_1) as l40_1.
+  destruct l40_1 as [|l40_1]. { discriminate. } symmetry in Heql40_1.
+  remember (translate_stmt B (cd_decls cd30) s30_2) as l40_2.
+  destruct l40_2 as [|l40_2]. { discriminate. } symmetry in Heql40_2.
+  assert (IHs30_1' := IHs30_1 l40_1 eq_refl). clear IHs30_1. rename IHs30_1' into IHs30_1.
+  assert (IHs30_2' := IHs30_2 l40_2 eq_refl). clear IHs30_2. rename IHs30_2' into IHs30_2.
+  inversion ok; subst l40; clear ok.
+  rewrite IHs30_1 with (loopinfo := loopinfo)
+                       (CallOk40 := L40.Callset.callset_descend_stmts_app_left eq_refl
+                                      (Callset.callset_descend_block eq_refl CallOk40)).
+  cbn. rewrite<- Heqinterpret_stmt_list.
+  assert (A: forall Ok1 Ok2 Ok3,
+    interpret_stmt_list world loc loopinfo (l40_1 ++ l40_2)%list Ok1
+     =
+    match interpret_stmt_list world loc loopinfo l40_1 Ok2
+    with
+    | (world', loc', StmtSuccess) =>
+        interpret_stmt_list world' loc' loopinfo l40_2 Ok3
+    | (world', loc', StmtAbort _ as result_a) | (world', loc', StmtReturnFromFunction _ as result_a) =>
+        (world', loc', result_a)
+    end).
+  {
+    clear Heql40_1 IHs30_1 Heql40_2 IHs30_2 CallOk40.
+    revert world loc.
+    induction l40_1 as [|h]; intros.
+    {
+      cbn in *.
+      assert (NilOk: forall OkNil,
+                       interpret_stmt_list world loc loopinfo nil OkNil
+                        =
+                       (world, loc, StmtSuccess))
+        by now rewrite Heqinterpret_stmt_list.
+      rewrite NilOk.
+      repeat f_equal; apply proof_irrelevance.
+    }
+    assert (Ok1': let _ := string_set_impl in
+                 FSet.is_subset (Callset.stmt_list_callset (h :: (l40_1 ++ l40_2)))
+                  (Callset.decl_callset (cached_translated_decl fc30 B CalldagOk FcNotVar)) = true)
+      by now rewrite List.app_comm_cons with (A := L40.AST.stmt).
+    replace (interpret_stmt_list world loc loopinfo ((h :: l40_1) ++ l40_2)%list Ok1)
+       with (interpret_stmt_list world loc loopinfo (h :: l40_1 ++ l40_2)%list Ok1').
+    2:{
+      revert Ok1 Ok1'. rewrite List.app_comm_cons with (A := L40.AST.stmt).
+      intros. repeat f_equal. apply proof_irrelevance.
+    }
+    rewrite Heqinterpret_stmt_list. cbn. rewrite<- Heqinterpret_stmt_list.
+    match goal with
+    |- context G [match ?interp bigger_call_depth_bound smaller_call_depth_bound Ebound cd40
+                                (translate_fun_ctx fc30 B CalldagOk FcNotVar)
+                                do_call_40 builtins world loc loopinfo h
+                                ?ok
+                  with _ => _ end] =>
+        remember interp as interpret_stmt; remember ok as OkH
+    end.
+    match goal with
+    |- context G [match interpret_stmt bigger_call_depth_bound smaller_call_depth_bound Ebound cd40
+                                       (translate_fun_ctx fc30 B CalldagOk FcNotVar)
+                                       do_call_40 builtins world loc loopinfo h
+                                       (L40.Callset.callset_descend_stmts_head eq_refl ?ok)
+                  with _ => _ end] =>
+        remember (L40.Callset.callset_descend_stmts_head eq_refl ok) as OkH'
+    end.
+    replace OkH' with OkH by apply proof_irrelevance.
+    destruct interpret_stmt as ((world', loc'), result).
+    now destruct result.
+  }
+  match goal with
+  |- _ = interpret_stmt_list world loc loopinfo (l40_1 ++ l40_2)%list ?ok =>
+      rewrite (A ok (L40.Callset.callset_descend_stmts_app_left eq_refl ok)
+                    (L40.Callset.callset_descend_stmts_app_right eq_refl ok))
+  end.
+  match goal with
+  |- context G [interpret_stmt_list world loc loopinfo l40_1 ?ok] =>
+      remember ok as ok1
+  end.
+  match goal with
+  |- context G [interpret_stmt_list world loc loopinfo l40_1
+                  (Callset.callset_descend_stmts_app_left _ ?ok)] =>
+      remember ok as ok2
+  end.
+  assert (ok1 = Callset.callset_descend_stmts_app_left eq_refl ok2)
+    by apply proof_irrelevance.
+  subst ok1.
+  assert (R: Callset.callset_descend_block eq_refl (Callset.callset_descend_stmts_app_left eq_refl ok2)
+              =
+             Callset.callset_descend_stmts_app_left eq_refl ok2)
+    by apply proof_irrelevance.
+  rewrite R.
+  destruct interpret_stmt_list as ((world', loc'), result).
+  destruct result; trivial.
+  rewrite IHs30_2 with (loopinfo := loopinfo)
+                       (CallOk40 := L40.Callset.callset_descend_stmts_app_right eq_refl
+                                      (Callset.callset_descend_block eq_refl CallOk40)).
+  cbn. rewrite<- Heqinterpret_stmt_list.
+  repeat f_equal. apply proof_irrelevance.
+}
+(* loop *)
+(* weird: cbn and simpl hang up on ok *)
+assert (CountNZ: Z_of_uint256 count <> 0%Z). (* translate_stmt raises an error if count = 0 *)
+{
+  unfold translate_stmt in ok.
+  intro CountZ.
+  rewrite<- Z.eqb_eq in CountZ.
+  rewrite CountZ in ok.
+  discriminate.
+}
+remember (translate_stmt B (cd_decls cd30) s30) as body40.
+unfold translate_stmt in ok. rewrite (proj2 (Z.eqb_neq _ _) CountNZ) in ok. fold translate_stmt in ok.
+rewrite<- Heqbody40 in ok.
+destruct body40 as [|body40]. { discriminate. }
+fold translate_stmt in Heqbody40.
+(* weird: inversion ok doesn't work, simple inversion doesn't work either *)
+assert (InvertInr: forall A B (x y: B) (H: @inr A B x = inr y),
+                     x = y).
+{ intros. now inversion H. }
+apply InvertInr in ok. clear InvertInr. (* why is it so hard for inversion? *)
+subst l40.
+(* cbn still hangs up *)
+unfold L40.Stmt.interpret_block.
+unfold BuiltinsSupportUInt256 in BuiltinsOk.
+assert (LtOk: BuiltinsSupportBinop builtins (builtin_name_uint256_lt B) UInt256.uint256_lt)
+  by tauto.
+assert (AddOk: BuiltinsSupportBinop builtins (builtin_name_uint256_add B)
+                 CheckedArith.uint256_add)
+  by tauto. (* used later for adding the counter to the offset *)
+clear BuiltinsOk.
+(* following CheckArith/Stmt here but that was about L30 so not using it directly *)
+remember (L40.Expr.interpret_expr _ _ _ _ _ _ _ _ _) as lt_result.
+unfold L40.Expr.interpret_expr in Heqlt_result.
+
+(* following do_binop from CheckArith/Stmt.v except we have a language with exprs now *)
+unfold BuiltinsSupportBinop in LtOk.
+destruct (builtins (builtin_name_uint256_lt B)) as [lt|]; try contradiction.
+assert (A := builtin_is_binop_arity _ _ LtOk).
+destruct lt as (lt_arity, lt).
+cbn in A.
+subst lt_arity.
+unfold Datatypes.length in Heqlt_result.
+rewrite if_yes with (E := Nat.eqb_refl 2) in Heqlt_result.
+rewrite (builtin_is_binop_ok _ _ LtOk) in Heqlt_result.
+subst lt_result. clear lt LtOk.
+unfold UInt256.uint256_lt.
+rewrite uint256_ok.
+rewrite Z.mod_small by (assert (Range := uint256_range count); lia).
+remember (2 ^ 256 - Z_of_uint256 count <? Z_of_uint256 (OpenArray.get loc var))%Z
+  as loop_is_bad.
+destruct loop_is_bad.
+{ (* loop overflows *)
+  replace (Z_of_uint256 one256 =? Z_of_uint256 zero256)%Z with false
+    by (unfold one256, zero256; now repeat rewrite uint256_ok).
+  cbn.
+  replace (Z_of_uint256 count =? 0)%Z with false
+    by (symmetry; now rewrite Z.eqb_neq).
+  enough (H: let _ := memory_impl in
+          (Z_of_uint256 (uint256_of_Z (Z_of_uint256 (OpenArray.get loc var) + Z_of_uint256 count - 1)) 
+            =?
+           Z_of_uint256 (OpenArray.get loc var) + Z_of_uint256 count - 1)%Z 
+            = false)
+    by now rewrite H.
+  clear IHs30 CallOk30 CallOk40 Heqbody40.
+  cbn.
+  rewrite uint256_ok.
+  rewrite Z.eqb_neq.
+  symmetry in Heqloop_is_bad. rewrite Z.ltb_lt in Heqloop_is_bad.
+  match goal with
+  |- ?l <> ?r => enough (H: (l < 2^256 <= r)%Z) by lia
+  end.
+  split. 2:lia.
+  now apply Z.mod_pos_bound.
+}
+(* no overflow *)
+symmetry in Heqloop_is_bad.
+rewrite Z.ltb_ge in Heqloop_is_bad.
+rename Heqloop_is_bad into NoOverflow.
+rewrite Z.eqb_refl.
+match goal with
+|- ?l = ?r => remember r as rhs
+end.
+cbn.
+replace (Z_of_uint256 count =? 0)%Z with false
+  by (symmetry; now rewrite Z.eqb_neq).
+replace ((Z_of_uint256 (uint256_of_Z (Z_of_uint256 (OpenArray.get loc var) + Z_of_uint256 count - 1)) 
+          =?
+         Z_of_uint256 (OpenArray.get loc var) + Z_of_uint256 count - 1)%Z)
+  with true.
+2:{
+  symmetry.
+  rewrite Z.eqb_eq.
+  rewrite uint256_ok.
+  apply Z.mod_small.
+  assert (R1 := let _ := memory_impl in uint256_range (OpenArray.get loc var)). cbn in R1.
+  assert (R2 := uint256_range count).
+  lia.
+}
+subst rhs.
+assert (R: forall x: world_state * memory * stmt_result uint256,
+          match x with
+          | (world', loc', StmtSuccess) => (world', loc', StmtSuccess)
+          | (world', loc', StmtAbort _ as result) | (world', loc', StmtReturnFromFunction _ as result) =>
+                (world', loc', result)
+          end = x)
+  by (destruct x as ((world', loc'), result); now destruct result).
+rewrite R. rewrite R.
+clear R.
+
+(* following CheckArith/Stmt here *)
+remember (let _ := memory_impl in
+          Z_of_uint256 (OpenArray.get loc var) + Z_of_uint256 count - 1)%Z as last.
+assert (LastRange: (0 <= last < 2 ^ 256)%Z).
+{
+  cbn in Heqlast.
+  subst.
+  assert (R1 := let _ := memory_impl in uint256_range (OpenArray.get loc var)). cbn in R1.
+  assert (R2 := uint256_range count).
+  lia.
+}
+
+(* L30 loop machinery: *)
+remember (Z.to_nat (Z_of_uint256 count)) as countdown.
+remember (Z_of_uint256 (OpenArray.get loc var)) as cursor.
+
+assert (MainLoopEq: last = (cursor + Z_of_uint256 count - 1)%Z)
+  by (subst cursor; exact Heqlast).
+
+(* L40 loop machinery: *)
+
+remember (OpenArray.get loc var) as this_loop_offset. (* unchanged during induction *)
+remember count as this_loop_count.                    (*           --//--           *)
+rewrite Heqthis_loop_count in MainLoopEq, Heqcountdown.
+rewrite Heqthis_loop_offset in Heqcursor.
+
+assert (MainLoopFixedEq: (last = Z_of_uint256 this_loop_offset + Z_of_uint256 this_loop_count - 1)%Z)
+  by now subst.
+
+assert (CountUpper: (Z_of_uint256 count <= Z_of_uint256 this_loop_count)%Z)
+  by (subst; apply Z.le_refl).
+
+clear Heqlast Heqcursor NoOverflow CountNZ Heqthis_loop_count Heqthis_loop_offset.
+revert count world loc cursor MainLoopEq CallOk30 CallOk40 Heqcountdown CountUpper.
+
+induction countdown. { trivial. }
+intros.
+remember (L40.Stmt.interpret_small_stmt _ _ _ _ world loc _ _ _) as iter_init.
+cbn in Heqiter_init.
+(* Now we need to do for add() the same things we did above for lt(). *)
+unfold BuiltinsSupportBinop in AddOk.
+destruct (builtins (builtin_name_uint256_add B)) as [sum|]; try contradiction.
+assert (A := builtin_is_binop_arity _ _ AddOk).
+destruct sum as (sum_arity, sum).
+cbn in A.
+subst sum_arity.
+unfold Datatypes.length in Heqiter_init.
+rewrite if_yes with (E := Nat.eqb_refl 2) in Heqiter_init.
+rewrite (builtin_is_binop_ok _ _ AddOk) in Heqiter_init.
+subst iter_init. clear sum AddOk.
+unfold CheckedArith.uint256_add.
+
+(* checking that the counter doesn't go below 0 *)
+pose (count' := uint256_of_Z (Z.pred (Z_of_uint256 count))).
+assert (CountOk: countdown = Z.to_nat (Z_of_uint256 count')).
+{
+  unfold count'. rewrite uint256_ok.
+  assert (R := uint256_range count).
+  remember (Z_of_uint256 count) as z. clear Heqz.
+  assert (W: z = Z.succ (Z.of_nat countdown)).
+  {
+    rewrite<- Nat2Z.inj_succ. rewrite Heqcountdown.
+    symmetry. apply Z2Nat.id. tauto.
+  }
+  subst z. rewrite Z.pred_succ.
+  replace (Z.of_nat countdown mod 2 ^ 256)%Z with (Z.of_nat countdown).
+  { symmetry. apply Nat2Z.id. }
+  symmetry. apply Z.mod_small.
+  split.
+  { (* 0 <= countdown *) apply Nat2Z.is_nonneg. }
+  exact (Z.lt_trans _ _ _ (Z.lt_succ_diag_r (Z.of_nat countdown)) (proj2 R)).
+}
+
+assert (CursorOk: cursor =
+           (Z_of_uint256 this_loop_offset +
+            Z_of_uint256 (uint256_of_Z (Z_of_uint256 this_loop_count - 1 - Z.of_nat countdown)))%Z).
+{
+  rewrite uint256_ok.
+  rewrite Z.mod_small
+    by (assert (R := uint256_range this_loop_count); lia).
+  lia.
+}
+rewrite<- CursorOk. (* now the L40 loop uses the same cursor as the L30 loop (for this iteration *)
+remember (OpenArray.put loc var (uint256_of_Z cursor))
+  as current_loc.
+remember ({|
+       Expr.loop_offset := this_loop_offset;
+       Expr.loop_count := this_loop_count;
+       Expr.loop_countdown := countdown
+     |} :: loopinfo)%list
+  as current_loopinfo.
+match goal with
+|- context G [ ?i_stmt_list world current_loc current_loopinfo body40 ?callok ] =>
+    remember i_stmt_list as do_stmt_list; remember callok as IterCallOk40
+end.
+rewrite (IHs30 body40 eq_refl) with (CallOk40 := IterCallOk40) (loopinfo := current_loopinfo).
+
+assert (R: Stmt.interpret_block Ebound (translate_fun_ctx fc30 B CalldagOk FcNotVar) do_call_40 builtins world
+            current_loc current_loopinfo (AST.Block body40) IterCallOk40
+           =
+          do_stmt_list world current_loc current_loopinfo body40 IterCallOk40).
+{
+  cbn.
+  rewrite Heqdo_stmt_list.
+  assert (E: @Callset.callset_descend_block C body40 (@AST.Block C body40)
+               (@Callset.decl_callset C
+                  (@cached_translated_decl C bigger_call_depth_bound cd30 fc30 cd40 B CalldagOk FcNotVar))
+               (@eq_refl (@AST.block C) (@AST.Block C body40)) IterCallOk40
+               =
+              IterCallOk40)
+    by apply proof_irrelevance.
+  rewrite E.
+  trivial.
+}
+rewrite R. clear R.
+
+assert (NextLoopEq: last = (Z.succ cursor + Z_of_uint256 count' - 1)%Z).
+{
+  subst count'.
+  rewrite uint256_ok.
+  rewrite Z.mod_small. { lia. }
+  assert (R := uint256_range count).
+  lia.
+}
+assert (NextCountUpper: (Z_of_uint256 count' <= Z_of_uint256 this_loop_count)%Z)
+  by lia.
+subst IterCallOk40.
+destruct do_stmt_list as ((world', loc'), result). (* finally we do the iteration *)
+destruct result; trivial.
+{
+  apply (IHcountdown count' world' loc' (Z.succ cursor) NextLoopEq
+                   CallOk30 CallOk40 CountOk NextCountUpper).
+}
+destruct a; trivial.
+apply (IHcountdown count' world' loc' (Z.succ cursor) NextLoopEq
+                 CallOk30 CallOk40 CountOk NextCountUpper).
+Qed.
